theories/Lambda/ExprDI.v
@@ -2,7 +2,6 @@ Require Import ExtLib.Structures.Monads.
 Require Import ExtLib.Data.HList.
 Require Import ExtLib.Data.Fun.
 Require Import ExtLib.Data.Monads.OptionMonad.
-Require Import ExtLib.Tactics.
 Require Import MirrorCore.SymI.
 Require Import MirrorCore.ExprI.
 Require Import MirrorCore.AbsAppI.
