theories/Lambda/ExprUnify_simul.v
@@ -1,6 +1,4 @@
-Require Import Coq.Lists.List.
 Require Import ExtLib.Core.RelDec.
-Require Import ExtLib.Data.ListNth.
 Require Import ExtLib.Data.HList.
 Require Import ExtLib.Data.Option.
 Require Import ExtLib.Data.Fun.
@@ -8,7 +6,6 @@ Require Import ExtLib.Data.Eq.
 Require Import ExtLib.Data.Pair.
 Require Import ExtLib.Tactics.
 Require Import MirrorCore.ExprI.
-Require Import MirrorCore.SymI.
 Require Import MirrorCore.SubstI.
 Require Import MirrorCore.UnifyI.
 Require Import MirrorCore.Lambda.ExprCore.
