theories/Views/EqView.v
@@ -1,15 +1,11 @@
 Require Import ExtLib.Core.RelDec.
 Require Import ExtLib.Data.Fun.
-Require Import ExtLib.Data.Map.FMapPositive.
-Require Import ExtLib.Data.SumN.
 Require Import ExtLib.Data.Positive.
 Require Import ExtLib.Tactics.Consider.
 Require Import ExtLib.Tactics.
 
 Require Import MirrorCore.TypesI.
-Require Import MirrorCore.syms.SymEnv.
-Require Import MirrorCore.syms.SymSum.
-Require Import MirrorCore.Lambda.Expr.
+Require Import MirrorCore.Lambda.ExprCore.
 Require Import MirrorCore.Lambda.Ptrns.
 Require Import MirrorCore.Views.Ptrns.
 Require Import MirrorCore.Views.FuncView.
@@ -25,10 +21,10 @@ Section EqFuncInst.
   Context {typ : Type} {RType_typ : RType typ}.
   Context {func : Type}.
   Context {Heq : RelDec (@eq typ)} {HC : RelDec_Correct Heq}.
-  
+
   Context {Typ2_tyArr : Typ2 _ Fun}.
   Context {Typ1_tyProp : Typ0 _ Prop}.
-  
+
   Let tyArr : typ -> typ -> typ := @typ2 _ _ _ Typ2_tyArr.
   Let tyProp : typ := @typ0 _ _ _ _.
 
@@ -42,13 +38,12 @@ Section EqFuncInst.
       | pEq t1, pEq t2 => Some (t1 ?[ eq ] t2)
     end.
 
-  Global Instance RelDec_eq_func : RelDec (@eq (eq_func typ)) := 
-    {
-      rel_dec a b := match eq_func_eq a b with 
-    	  	       | Some b => b 
-    		       | None => false 
-    		     end
-    }.
+  Global Instance RelDec_eq_func : RelDec (@eq (eq_func typ)) :=
+  { rel_dec a b := match eq_func_eq a b with
+    	  	   | Some b => b
+    		   | None => false
+    		   end
+  }.
 
   Definition eqR t : typD (tyArr t (tyArr t tyProp)) :=
     castR id (Fun (typD t) (Fun (typD t) Prop)) (@eq (typD t)).
@@ -61,12 +56,11 @@ Section EqFuncInst.
       | pEq t => eqR t
     end.
 
-  Global Instance RSym_EqFunc : SymI.RSym (eq_func typ) := 
-    {
-      typeof_sym := typeof_eq_func;
-      symD := eq_func_symD;
-      sym_eqb := eq_func_eq
-    }.
+  Global Instance RSym_EqFunc : SymI.RSym (eq_func typ) :=
+  { typeof_sym := typeof_eq_func;
+    symD := eq_func_symD;
+    sym_eqb := eq_func_eq
+  }.
 
   Global Instance RSymOk_EqFunc : SymI.RSymOk RSym_EqFunc.
   Proof.
@@ -79,10 +73,11 @@ End EqFuncInst.
 
 Section MakeEq.
   Context {typ func : Type} {FV : FuncView func (eq_func typ)}.
-  
+
   Definition fEq t := f_insert (pEq t).
 
-  Definition mkCons (t : typ) (a b : expr typ func) := App (App (Inj (fEq t)) a) b.
+  Definition mkCons (t : typ) (a b : expr typ func) :=
+    App (App (Inj (fEq t)) a) b.
 
   Definition fptrnEq {T : Type} (p : Ptrns.ptrn typ T) : ptrn (eq_func typ) T :=
     fun f U good bad =>
@@ -115,12 +110,12 @@ Section MakeEq.
     exists t; split; [assumption | reflexivity].
   Qed.
 
-  Global Instance fptrnEq_SucceedsE {T : Type} {f : eq_func typ} 
-         {p : ptrn typ T} {res : T} {pok : ptrn_ok p} :
-    SucceedsE f (fptrnEq p) res := {
-      s_result := exists t, Succeeds t p res /\ f = pEq t;
-      s_elim := @Succeeds_fptrnEq T f p res pok
-    }.
+  Global Instance fptrnEq_SucceedsE {T : Type} {f : eq_func typ}
+         {p : ptrn typ T} {res : T} {pok : ptrn_ok p}
+  : SucceedsE f (fptrnEq p) res :=
+  { s_result := exists t, Succeeds t p res /\ f = pEq t;
+    s_elim := @Succeeds_fptrnEq T f p res pok
+  }.
 
 End MakeEq.
 
@@ -128,12 +123,12 @@ Section PtrnEq.
   Context {typ func : Type} {RType_typ : RType typ}.
   Context {FV : FuncView func (eq_func typ)}.
 
-(* Putting this in the previous sectioun caused universe inconsistencies 
+(* Putting this in the previous sectioun caused universe inconsistencies
   when calling '@mkEq typ func' in JavaFunc (with typ and func instantiated) *)
 
   Definition ptrnEq {A B T : Type}
              (p : ptrn typ T)
-             (a : ptrn (expr typ func) A) 
+             (a : ptrn (expr typ func) A)
              (b : ptrn (expr typ func) B) : ptrn (expr typ func) (T * A * B) :=
     app (app (inj (ptrn_view _ (fptrnEq p))) a) b.
 
