theories/Views/ListOpView.v
@@ -1,14 +1,9 @@
 Require Import ExtLib.Core.RelDec.
 Require Import ExtLib.Data.Fun.
-Require Import ExtLib.Data.Map.FMapPositive.
-Require Import ExtLib.Data.SumN.
-Require Import ExtLib.Data.Positive.
 Require Import ExtLib.Tactics.Consider.
 Require Import ExtLib.Tactics.
 
 Require Import MirrorCore.TypesI.
-Require Import MirrorCore.syms.SymEnv.
-Require Import MirrorCore.syms.SymSum.
 Require Import MirrorCore.Lambda.Expr.
 Require Import MirrorCore.Lambda.Ptrns.
 Require Import MirrorCore.Lambda.Red.
@@ -25,26 +20,26 @@ Set Strict Implicit.
 Set Maximal Implicit Insertion.
 
 Inductive listOp_func (typ : Type) :=
-  | pLength : typ -> listOp_func typ
-  | pNoDup : typ -> listOp_func typ
-  | pIn : typ -> listOp_func typ
-  | pMap : typ -> typ -> listOp_func typ
-  | pFold : typ -> typ -> listOp_func typ
-  | pCombine : typ -> typ -> listOp_func typ.
+| pLength : typ -> listOp_func typ
+| pNoDup : typ -> listOp_func typ
+| pIn : typ -> listOp_func typ
+| pMap : typ -> typ -> listOp_func typ
+| pFold : typ -> typ -> listOp_func typ
+| pCombine : typ -> typ -> listOp_func typ.
 
 Section ListOpFuncInst.
   Context {typ : Type} {RType_typ : RType typ}.
   Context {func : Type}.
   Context {Heq : RelDec (@eq typ)} {HC : RelDec_Correct Heq}.
-  
+
   Context {Typ2_tyArr : Typ2 _ Fun}.
   Context {Typ2_tyProd : Typ2 _ prod}.
   Context {Typ1_tyList : Typ1 _ list}.
   Context {Typ0_tyProp : Typ0 _ Prop}.
   Context {Typ0_tyNat : Typ0 _ nat}.
-  
+
   Context {Typ0_tyPropOk : Typ0Ok Typ0_tyProp}.
-  
+
   Let tyArr : typ -> typ -> typ := @typ2 _ _ _ Typ2_tyArr.
   Let tyProd : typ -> typ -> typ := @typ2 _ _ _ Typ2_tyProd.
   Let tyList : typ -> typ := @typ1 _ _ _ Typ1_tyList.
@@ -53,12 +48,14 @@ Section ListOpFuncInst.
 
   Definition typeof_listOp_func lf :=
     match lf with
-      | pLength t => Some (tyArr (tyList t) tyNat)
-      | pNoDup t => Some (tyArr (tyList t) tyProp)
-      | pIn t => Some (tyArr t (tyArr (tyList t) tyProp))
-      | pMap t1 t2 => Some (tyArr (tyArr t1 t2) (tyArr (tyList t1) (tyList t2)))
-      | pFold t1 t2 => Some (tyArr (tyArr t2 (tyArr t1 t1)) (tyArr t1 (tyArr (tyList t2) t1))) 
-      | pCombine t1 t2 => Some (tyArr (tyList t1) (tyArr (tyList t2) (tyList (tyProd t1 t2))))
+    | pLength t => Some (tyArr (tyList t) tyNat)
+    | pNoDup t => Some (tyArr (tyList t) tyProp)
+    | pIn t => Some (tyArr t (tyArr (tyList t) tyProp))
+    | pMap t1 t2 => Some (tyArr (tyArr t1 t2) (tyArr (tyList t1) (tyList t2)))
+    | pFold t1 t2 =>
+      Some (tyArr (tyArr t2 (tyArr t1 t1)) (tyArr t1 (tyArr (tyList t2) t1)))
+    | pCombine t1 t2 =>
+      Some (tyArr (tyList t1) (tyArr (tyList t2) (tyList (tyProd t1 t2))))
     end.
 
   Definition listOp_func_eq (a b : listOp_func typ) : option bool :=
@@ -75,34 +72,34 @@ Section ListOpFuncInst.
       | _, _ => None
     end.
 
-  Global Instance RelDec_list_func : RelDec (@eq (listOp_func typ)) := 
+  Global Instance RelDec_list_func : RelDec (@eq (listOp_func typ)) :=
     {
-      rel_dec a b := match listOp_func_eq a b with 
-    	  	       | Some b => b 
-    		       | None => false 
+      rel_dec a b := match listOp_func_eq a b with
+    	  	       | Some b => b
+    		       | None => false
     		     end
     }.
 
-  Definition lengthR t : typD (tyArr (tyList t) tyNat) := 
+  Definition lengthR t : typD (tyArr (tyList t) tyNat) :=
     castR id (Fun (list (typD t)) nat) (@length (typD t)).
 
   Definition NoDupR t : typD (tyArr (tyList t) tyProp) :=
     castR id (Fun (list (typD t)) Prop) (@NoDup (typD t)).
-  
-  Definition InR t : typD (tyArr t (tyArr (tyList t) tyProp)) := 
+
+  Definition InR t : typD (tyArr t (tyArr (tyList t) tyProp)) :=
     castR id (Fun (typD t) (Fun (list (typD t)) Prop)) (@In (typD t)).
 
   Definition mapR t u : typD (tyArr (tyArr t u) (tyArr (tyList t) (tyList u))) :=
-    castR id (Fun (Fun (typD t) (typD u)) (Fun (list (typD t)) (list (typD u)))) 
+    castR id (Fun (Fun (typD t) (typD u)) (Fun (list (typD t)) (list (typD u))))
           (@map (typD t) (typD u)).
 
   Definition foldR t u : typD (tyArr (tyArr u (tyArr t t)) (tyArr t (tyArr (tyList u) t))) :=
-    castR id (Fun (Fun (typD u) (Fun (typD t) (typD t))) 
-                  (Fun (typD t) (Fun (list (typD u)) (typD t)))) 
+    castR id (Fun (Fun (typD u) (Fun (typD t) (typD t)))
+                  (Fun (typD t) (Fun (list (typD u)) (typD t))))
           (@fold_right (typD t) (typD u)).
 
   Definition combineR t u : typD (tyArr (tyList t) (tyArr (tyList u) (tyList (tyProd t u)))) :=
-    castR id (Fun (list (typD t)) (Fun (list (typD u)) (list ((typD t) * (typD u))))) 
+    castR id (Fun (list (typD t)) (Fun (list (typD u)) (list ((typD t) * (typD u)))))
           (@combine (typD t) (typD u)).
 
   Definition listOp_func_symD lf :=
@@ -118,7 +115,7 @@ Section ListOpFuncInst.
       | pCombine t1 t2 => combineR t1 t2
     end.
 
-  Global Instance RSym_ListOpFunc : SymI.RSym (listOp_func typ) := 
+  Global Instance RSym_ListOpFunc : SymI.RSym (listOp_func typ) :=
     {
       typeof_sym := typeof_listOp_func;
       symD := listOp_func_symD;
@@ -132,9 +129,9 @@ Section ListOpFuncInst.
     + consider (t ?[ eq ] t0); intuition congruence.
     + consider (t ?[ eq ] t0); intuition congruence.
     + consider (t ?[ eq ] t0); intuition congruence.
-    + consider (t ?[ eq ] t1 && t0 ?[ eq ] t2)%bool; intuition congruence. 
-    + consider (t ?[ eq ] t1 && t0 ?[ eq ] t2)%bool; intuition congruence. 
-    + consider (t ?[ eq ] t1 && t0 ?[ eq ] t2)%bool; intuition congruence. 
+    + consider (t ?[ eq ] t1 && t0 ?[ eq ] t2)%bool; intuition congruence.
+    + consider (t ?[ eq ] t1 && t0 ?[ eq ] t2)%bool; intuition congruence.
+    + consider (t ?[ eq ] t1 && t0 ?[ eq ] t2)%bool; intuition congruence.
   Qed.
 
 End ListOpFuncInst.
@@ -149,22 +146,22 @@ Section MakeListOp.
   Definition fFold t u := f_insert (pFold t u).
   Definition fCombine t u := f_insert (pCombine t u).
 
-  Definition mkLength t (lst : expr typ func) : expr typ func := 
+  Definition mkLength t (lst : expr typ func) : expr typ func :=
     App (Inj (fLength t)) lst.
 
-  Definition mkNoDup t (lst : expr typ func) : expr typ func := 
+  Definition mkNoDup t (lst : expr typ func) : expr typ func :=
     App (Inj (fNoDup t)) lst.
 
-  Definition mkIn t (lst : expr typ func) : expr typ func := 
+  Definition mkIn t (lst : expr typ func) : expr typ func :=
     App (Inj (fIn t)) lst.
 
-  Definition mkMap t u (f lst : expr typ func) : expr typ func := 
+  Definition mkMap t u (f lst : expr typ func) : expr typ func :=
     App (App (Inj (fMap t u)) f) lst.
 
-  Definition mkFold t u (f acc lst : expr typ func) : expr typ func := 
+  Definition mkFold t u (f acc lst : expr typ func) : expr typ func :=
     App (App (App (Inj (fFold t u)) f) acc) lst.
 
-  Definition mkCombine t u (xs ys : expr typ func) : expr typ func := 
+  Definition mkCombine t u (xs ys : expr typ func) : expr typ func :=
     App (App (Inj (fCombine t u)) xs) ys.
 
   Definition fptrnLength {T : Type} (p : Ptrns.ptrn typ T) : ptrn (listOp_func typ) T :=
@@ -286,7 +283,7 @@ Section MakeListOp.
       rewrite H. reflexivity. }
     { right; unfold Fails in *; intros; simpl; rewrite H; reflexivity. }
   Qed.
-  
+
   Lemma Succeeds_fptrnLength {T : Type} (f : listOp_func typ) (p : ptrn typ T) (res : T)
         {pok : ptrn_ok p} (H : Succeeds f (fptrnLength p) res) :
     exists t, Succeeds t p res /\ f = pLength t.
@@ -376,56 +373,56 @@ Section MakeListOp.
     rewrite H0 in H; inv_all; subst.
     exists t, t0; split; [assumption | reflexivity].
   Qed.
-  
-  Global Instance fptrnLength_SucceedsE {T : Type} {f : listOp_func typ} 
+
+  Global Instance fptrnLength_SucceedsE {T : Type} {f : listOp_func typ}
          {p : ptrn typ T} {res : T} {pok : ptrn_ok p} :
     SucceedsE f (fptrnLength p) res := {
       s_result := exists t, Succeeds t p res /\ f = pLength t;
       s_elim := @Succeeds_fptrnLength T f p res pok
     }.
 
-  Global Instance fptrnNoDup_SucceedsE {T : Type} {f : listOp_func typ} 
+  Global Instance fptrnNoDup_SucceedsE {T : Type} {f : listOp_func typ}
          {p : ptrn typ T} {res : T} {pok : ptrn_ok p} :
     SucceedsE f (fptrnNoDup p) res := {
       s_result := exists t, Succeeds t p res /\ f = pNoDup t;
       s_elim := @Succeeds_fptrnNoDup T f p res pok
     }.
 
-  Global Instance fptrnIn_SucceedsE {T : Type} {f : listOp_func typ} 
+  Global Instance fptrnIn_SucceedsE {T : Type} {f : listOp_func typ}
          {p : ptrn typ T} {res : T} {pok : ptrn_ok p} :
     SucceedsE f (fptrnIn p) res := {
       s_result := exists t, Succeeds t p res /\ f = pIn t;
       s_elim := @Succeeds_fptrnIn T f p res pok
     }.
 
-  Global Instance fptrnMap_SucceedsE {T : Type} {f : listOp_func typ} 
+  Global Instance fptrnMap_SucceedsE {T : Type} {f : listOp_func typ}
          {p : ptrn (typ * typ) T} {res : T} {pok : ptrn_ok p} :
     SucceedsE f (fptrnMap p) res := {
       s_result := exists t u, Succeeds (t, u) p res /\ f = pMap t u;
       s_elim := @Succeeds_fptrnMap T f p res pok
     }.
 
-  Global Instance fptrnFold_SucceedsE {T : Type} {f : listOp_func typ} 
+  Global Instance fptrnFold_SucceedsE {T : Type} {f : listOp_func typ}
          {p : ptrn (typ * typ) T} {res : T} {pok : ptrn_ok p} :
     SucceedsE f (fptrnFold p) res := {
       s_result := exists t u, Succeeds (t, u) p res /\ f = pFold t u;
       s_elim := @Succeeds_fptrnFold T f p res pok
     }.
 
-  Global Instance fptrnCombine_SucceedsE {T : Type} {f : listOp_func typ} 
+  Global Instance fptrnCombine_SucceedsE {T : Type} {f : listOp_func typ}
          {p : ptrn (typ * typ) T} {res : T} {pok : ptrn_ok p} :
     SucceedsE f (fptrnCombine p) res := {
       s_result := exists t u, Succeeds (t, u) p res /\ f = pCombine t u;
       s_elim := @Succeeds_fptrnCombine T f p res pok
     }.
-	
+
 End MakeListOp.
 
 Section PtrnListOp.
   Context {typ func : Type} {RType_typ : RType typ}.
   Context {FV : FuncView func (listOp_func typ)}.
 
-(* Putting this in the previous sectioun caused universe inconsistencies 
+(* Putting this in the previous sectioun caused universe inconsistencies
   when calling '@mkLength typ func' in JavaFunc (with typ and func instantiated) *)
 
   Definition ptrnLength {T A : Type}
@@ -441,18 +438,18 @@ Section PtrnListOp.
     app (inj (ptrn_view _ (fptrnIn p))) a.
 
   Definition ptrnMap {T A B : Type}
-             (p : ptrn (typ * typ) T) (a : ptrn (expr typ func) A) 
+             (p : ptrn (typ * typ) T) (a : ptrn (expr typ func) A)
              (b : ptrn (expr typ func) B) : ptrn (expr typ func) (T * A * B) :=
     app (app (inj (ptrn_view _ (fptrnMap p))) a) b.
-  
+
   Definition ptrnFold {T A B C : Type}
-             (p : ptrn (typ * typ) T) (a : ptrn (expr typ func) A) 
-             (b : ptrn (expr typ func) B) (c : ptrn (expr typ func) C) : 
+             (p : ptrn (typ * typ) T) (a : ptrn (expr typ func) A)
+             (b : ptrn (expr typ func) B) (c : ptrn (expr typ func) C) :
     ptrn (expr typ func) (T * A * B * C) :=
     app (app (app (inj (ptrn_view _ (fptrnFold p))) a) b) c.
-  
+
   Definition ptrnCombine {T A B : Type}
-             (p : ptrn (typ * typ) T) (a : ptrn (expr typ func) A) 
+             (p : ptrn (typ * typ) T) (a : ptrn (expr typ func) A)
              (b : ptrn (expr typ func) B) : ptrn (expr typ func) (T * A * B) :=
     app (app (inj (ptrn_view _ (fptrnCombine p))) a) b.
 
@@ -478,7 +475,7 @@ Section Tactics.
   Context {FVOk_list : FuncViewOk (typ := typ) FV_list RSym_func RSym_ListFunc}.
   Context {FVOk_nat : FuncViewOk (typ := typ) FV_nat RSym_func RSym_NatFunc}.
   Context {FVOk_prod : FuncViewOk (typ := typ) FV_prod RSym_func RSym_ProdFunc}.
-  
+
   Let tyArr : typ -> typ -> typ := @typ2 _ _ _ Typ2_tyArr.
   Let tyProd : typ -> typ -> typ := @typ2 _ _ _ Typ2_tyProd.
   Let tyList : typ -> typ := @typ1 _ _ _ Typ1_tyList.
@@ -486,23 +483,23 @@ Section Tactics.
   Let tyNat : typ := @typ0 _ _ _ Typ0_tyNat.
 
   Fixpoint lst_length (lst : expr typ func) (t : typ) (acc : nat) : expr typ func :=
-    run_tptrn 
-      (list_cases 
+    run_tptrn
+      (list_cases
          (fun _ => mkNat acc)
          (fun _ _ lst => (lst_length lst t (S acc)))
          (mkPlus (mkLength t lst) (mkNat acc))) lst.
-    
-  Lemma lst_length_unfold (lst : expr typ func) (t : typ) (acc : nat) : 
-    lst_length lst t acc = 
-    run_tptrn 
-      (list_cases 
+
+  Lemma lst_length_unfold (lst : expr typ func) (t : typ) (acc : nat) :
+    lst_length lst t acc =
+    run_tptrn
+      (list_cases
          (fun _ => mkNat acc)
          (fun _ _ lst => (lst_length lst t (S acc)))
          (mkPlus (mkLength t lst) (mkNat acc))) lst.
   Proof.
     destruct lst; simpl; reflexivity.
   Qed.
-    
+
   Definition red_length_ptrn : ptrn (expr typ func) (expr typ func) :=
     pmap (fun x => lst_length (snd x) (fst x) 0) (ptrnLength get get).
 
@@ -567,17 +564,16 @@ Section Tactics.
     run_tptrn
       (@list_cases typ func FV_list (expr typ func)
          (fun _ => @mkNil typ func FV_list (tyProd t u))
-         (fun _ x xs' => 
-            run_tptrn 
+         (fun _ x xs' =>
+            run_tptrn
               (@list_cases typ func FV_list (expr typ func)
                  (fun _ => @mkNil typ func FV_list (tyProd t u))
-                 (fun _ y ys' => @mkCons typ func FV_list (tyProd t u) 
-                                         (@mkPair typ func FV_prod t u x y) 
-                                        (TODO xs' ys' t u)) 
+                 (fun _ y ys' => @mkCons typ func FV_list (tyProd t u)
+                                         (@mkPair typ func FV_prod t u x y)
+                                        (TODO xs' ys' t u))
                  (@mkCombine typ func FV_listOp t u xs ys)) ys)
          (@mkCombine typ func FV_listOp t u xs ys)) xs.
 
-Print lst_combine.
 Eval unfold lst_combine, list_cases, run_tptrn, pdefault, por, pmap,
   ptrnNil, ptrnCons, app, inj, Mmap, Mrebuild, Mbind, ptrn_view, fptrnCons, fptrnNil, get in lst_combine.
 *)
@@ -588,7 +584,7 @@ Eval unfold lst_combine, list_cases, run_tptrn, pdefault, por, pmap,
                            (fun _ x xs => mkCons u (beta (App f x)) (red_map_ptrn t u f xs))
                            (mkMap t u f lst)) lst.
 
-  Lemma red_map_unfold (t u : typ) (f lst : expr typ func) : 
+  Lemma red_map_unfold (t u : typ) (f lst : expr typ func) :
     red_map_ptrn t u f lst =
     run_tptrn (@list_cases typ func _ _
                            (fun _ => mkNil u)
@@ -596,9 +592,9 @@ Eval unfold lst_combine, list_cases, run_tptrn, pdefault, por, pmap,
                            (mkMap t u f lst)) lst.
   Proof.
     destruct lst; simpl; reflexivity.
-  Qed.    
+  Qed.
 
-  Definition red_map := 
+  Definition red_map :=
     run_tptrn (pdefault_id (pmap (fun x => match x with
                                              | ((t, u), f, lst) => red_map_ptrn t u f lst
                                            end) (ptrnMap get get get))).
@@ -607,36 +603,36 @@ Eval unfold lst_combine, list_cases, run_tptrn, pdefault, por, pmap,
   Fixpoint red_fold_ptrn t u (f acc lst : expr typ func) : expr typ func :=
     run_tptrn (@list_cases typ func _ _
                            (fun _ => acc)
-                           (fun _ x xs => 
+                           (fun _ x xs =>
                               beta (beta (App (App f x) (red_fold_ptrn t u f acc xs))))
                            (mkFold t u f acc lst)) lst.
 
-  Lemma red_fold_unfold (t u : typ) (f acc lst : expr typ func) : 
+  Lemma red_fold_unfold (t u : typ) (f acc lst : expr typ func) :
     red_fold_ptrn t u f acc lst =
     run_tptrn (@list_cases typ func _ _
                            (fun _ => acc)
-                           (fun _ x xs => 
+                           (fun _ x xs =>
                               beta (beta (App (App f x) (red_fold_ptrn t u f acc xs))))
                            (mkFold t u f acc lst)) lst.
 
   Proof.
     destruct lst; simpl; reflexivity.
-  Qed.    
+  Qed.
 
-  Definition red_fold := 
+  Definition red_fold :=
     run_tptrn (pdefault_id (pmap (fun x => match x with
-                                             | ((t, u), f, acc, lst) => 
+                                             | ((t, u), f, acc, lst) =>
                                                red_fold_ptrn t u f acc lst
                                            end) (ptrnFold get get get get))).
 
 
 
 
-  Lemma lst_length_sound tus tvs (t : typ) (lst : expr typ func) 
+  Lemma lst_length_sound tus tvs (t : typ) (lst : expr typ func)
         (x : exprT tus tvs (typD (tyList t))) (n : nat)
         (H : ExprDsimul.ExprDenote.exprD' tus tvs (tyList t) lst = Some x) :
-    ExprDsimul.ExprDenote.exprD' tus tvs tyNat (lst_length lst t n) = 
-    Some (castR (exprT tus tvs) nat 
+    ExprDsimul.ExprDenote.exprD' tus tvs tyNat (lst_length lst t n) =
+    Some (castR (exprT tus tvs) nat
                 (fun us vs => length (castD (exprT tus tvs)
                                             (list (typD t)) x us vs) + n)).
   Proof.
@@ -646,7 +642,7 @@ Eval unfold lst_combine, list_cases, run_tptrn, pdefault, por, pmap,
     unfold run_tptrn, list_cases.
     apply pdefault_sound; [apply _ | | intros; ptrnE; destruct H1; ptrnE |].
     { intros a b Hab c d Hcd; subst; erewrite Hcd; reflexivity. }
-    { unfold nilR, mkNat, fNat, ptret. solve_denotation. 
+    { unfold nilR, mkNat, fNat, ptret. solve_denotation.
       unfold natR. solve_denotation. reflexivity. }
     { unfold ptret, consR. solve_denotation; simpl.
       erewrite H; [| eauto with acc_db | eassumption].
@@ -661,14 +657,14 @@ Eval unfold lst_combine, list_cases, run_tptrn, pdefault, por, pmap,
       reflexivity.
     }
   Qed.
-    
+
   Lemma red_length_ok : partial_reducer_ok (fun e args => red_length (apps e args)).
   Proof.
     unfold partial_reducer_ok; intros.
     exists val; split; [|reflexivity].
     generalize dependent (apps e es); clear e es; intros e H.
     unfold red_length.
-  
+
     apply run_tptrn_id_sound; [assumption|]; intros.
     unfold red_length_ptrn in H0.
     solve_denotation.
@@ -678,12 +674,12 @@ Eval unfold lst_combine, list_cases, run_tptrn, pdefault, por, pmap,
     repeat f_equal. do 2 (apply functional_extensionality; intros). omega.
   Qed.
 
-  Lemma map_ptrn_ok tus tvs (t u : typ) (f lst : expr typ func) 
+  Lemma map_ptrn_ok tus tvs (t u : typ) (f lst : expr typ func)
         (df : exprT tus tvs (typD (tyArr t u)))
         (dlst : exprT tus tvs (typD (tyList t)))
-        (Hf : ExprDsimul.ExprDenote.exprD' tus tvs (tyArr t u) f = Some df) 
+        (Hf : ExprDsimul.ExprDenote.exprD' tus tvs (tyArr t u) f = Some df)
         (Hlst : ExprDsimul.ExprDenote.exprD' tus tvs (tyList t) lst = Some dlst) :
-    ExprDsimul.ExprDenote.exprD' tus tvs (tyList u) (red_map_ptrn t u f lst) = 
+    ExprDsimul.ExprDenote.exprD' tus tvs (tyList u) (red_map_ptrn t u f lst) =
     Some (castR (exprT tus tvs) (list (typD u))
                 (fun vs us =>
                    map (castD (exprT tus tvs) (Fun (typD t) (typD u)) df vs us)
@@ -724,14 +720,14 @@ Eval unfold lst_combine, list_cases, run_tptrn, pdefault, por, pmap,
     erewrite map_ptrn_ok; [reflexivity | eassumption | eassumption].
   Qed.
 
-  Lemma fold_ptrn_ok tus tvs (t u : typ) (f acc lst : expr typ func) 
+  Lemma fold_ptrn_ok tus tvs (t u : typ) (f acc lst : expr typ func)
         (df : exprT tus tvs (typD (tyArr u (tyArr t t))))
         (dacc : exprT tus tvs (typD t))
         (dlst : exprT tus tvs (typD (tyList u)))
-        (Hf : ExprDsimul.ExprDenote.exprD' tus tvs (tyArr u (tyArr t t)) f = Some df) 
-        (HAcc : ExprDsimul.ExprDenote.exprD' tus tvs t acc = Some dacc) 
+        (Hf : ExprDsimul.ExprDenote.exprD' tus tvs (tyArr u (tyArr t t)) f = Some df)
+        (HAcc : ExprDsimul.ExprDenote.exprD' tus tvs t acc = Some dacc)
         (Hlst : ExprDsimul.ExprDenote.exprD' tus tvs (tyList u) lst = Some dlst) :
-    ExprDsimul.ExprDenote.exprD' tus tvs t (red_fold_ptrn t u f acc lst) = 
+    ExprDsimul.ExprDenote.exprD' tus tvs t (red_fold_ptrn t u f acc lst) =
     Some (castR (exprT tus tvs) (typD t)
                 (fun vs us =>
                    fold_right (castD (exprT tus tvs) (Fun (typD u) (Fun (typD t) (typD t))) df vs us)
@@ -739,7 +735,7 @@ Eval unfold lst_combine, list_cases, run_tptrn, pdefault, por, pmap,
                               (castD (exprT tus tvs) (list (typD u)) dlst vs us))).
   Proof.
     Opaque beta.
-    revert Hlst. generalize dependent dlst. 
+    revert Hlst. generalize dependent dlst.
     apply expr_strong_ind_no_case with (e := lst); intros.
     rewrite red_fold_unfold.
     unfold run_tptrn, list_cases.
@@ -751,7 +747,7 @@ Eval unfold lst_combine, list_cases, run_tptrn, pdefault, por, pmap,
 
     { unfold ptret. solve_denotation.
       eapply H; [eauto with acc_db | eassumption].
-      unfold consR. solve_denotation. 
+      unfold consR. solve_denotation.
       solve_denotation.
       reflexivity. }
     { unfold ptret, mkFold, fFold.
